LeanYjs/Totality.lean
@@ -14,7 +14,7 @@ import LeanYjs.ItemSet
   obtain ⟨ p, ⟨ hp, hp', hp'', hp''' ⟩ ⟩ := P
   assumption
 
-lemma yjs_lt_total {A : Type} {P : @ClosedPredicate A} {inv : ItemSetInvariant P} {x y : YjsPtr A} (hx : P.val x) (hy : P.val y) :
+lemma yjs_lt_total {A : Type} {P : ClosedPredicate A} {inv : ItemSetInvariant P} {x y : YjsPtr A} (hx : P.val x) (hy : P.val y) :
   (∃ h, @YjsLeq A P h x y) ∨ (∃ h, @YjsLt A P h y x) :=
   match x with
   | YjsPtr.first =>
@@ -75,6 +75,7 @@ lemma yjs_lt_total {A : Type} {P : @ClosedPredicate A} {inv : ItemSetInvariant P
     | YjsPtr.itemPtr y => by
       obtain ⟨ xo, xr, xid, xc ⟩ := x
       obtain ⟨ yo, yr, yid, yc ⟩ := y
+      unfold ClosedPredicate at *
       have hxo : P.val xo := by
         apply origin_p_valid (YjsItem.item xo xr xid xc) hx
       have hyo : P.val yo := by
@@ -83,42 +84,42 @@ lemma yjs_lt_total {A : Type} {P : @ClosedPredicate A} {inv : ItemSetInvariant P
         apply right_origin_p_valid (YjsItem.item xo xr xid xc) hx
       have hyr : P.val yr := by
         apply right_origin_p_valid (YjsItem.item yo yr yid yc) hy
-      obtain hleq := yjs_lt_total hx hyo
+      obtain hleq := yjs_lt_total hx hyo (inv := inv)
       cases hleq with
       | inl hleq =>
         obtain ⟨ h, hleq ⟩ := hleq
         left
-        suffices (∃ h, YjsLt P h (YjsPtr.itemPtr (YjsItem.item xo xr xid xc)) (YjsPtr.itemPtr (YjsItem.item yo yr yid yc))) from by
+        suffices (∃ h, YjsLt _ h (YjsPtr.itemPtr (YjsItem.item xo xr xid xc)) (YjsPtr.itemPtr (YjsItem.item yo yr yid yc))) from by
           obtain ⟨ h, hlt ⟩ := this
           exists h
           right
           assumption
         apply yjs_leq_p_trans1 inv _ _ _ _ 0 hleq _
         apply YjsLt.ltOriginOrder
-        apply OriginLt.ltOrigin <;> try first | simp | assumption
+        apply OriginLt.ltOrigin <;> try first | assumption | simp
         apply OriginLtStep.lt_left
       | inr hltyox =>
-        obtain hleq := yjs_lt_total hyr hx
+        obtain hleq := yjs_lt_total hyr hx (inv := inv)
         cases hleq with
         | inl hleq =>
           obtain ⟨ h, hleq ⟩ := hleq
           right
           apply yjs_leq_p_trans2 inv _ _ _ 0 _ _ hleq
           apply YjsLt.ltOriginOrder
-          apply OriginLt.ltOrigin <;> try first | simp | assumption
+          apply OriginLt.ltOrigin <;> try first | assumption | simp
           apply OriginLtStep.lt_right
         | inr hltxyr =>
-          obtain hleq := yjs_lt_total hy hxo
+          obtain hleq := yjs_lt_total hy hxo (inv := inv)
           cases hleq with
           | inl hleq =>
             obtain ⟨ h, hleq ⟩ := hleq
             right
             apply yjs_leq_p_trans1 inv _ _ _ _ 0 hleq _
             apply YjsLt.ltOriginOrder
-            apply OriginLt.ltOrigin <;> try first | simp | assumption
+            apply OriginLt.ltOrigin <;> try first | assumption | simp
             apply OriginLtStep.lt_left
           | inr hltxoy =>
-            obtain hleq := yjs_lt_total hxr hy
+            obtain hleq := yjs_lt_total hxr hy (inv := inv)
             cases hleq with
             | inl hleq =>
               obtain ⟨ h, hleq ⟩ := hleq
@@ -126,14 +127,14 @@ lemma yjs_lt_total {A : Type} {P : @ClosedPredicate A} {inv : ItemSetInvariant P
               apply yjs_leq_p_trans inv _ _ _ 0 _ _ hleq
               right
               apply YjsLt.ltOriginOrder
-              apply OriginLt.ltOrigin <;> try first | simp | assumption
+              apply OriginLt.ltOrigin <;> try first | assumption | simp
               apply OriginLtStep.lt_right
             | inr hltyxr =>
               obtain ⟨ h1, hlt_yo_x ⟩ := hltyox
               obtain ⟨ h2, hlt_x_yo ⟩ := hltxoy
               obtain ⟨ h3, hlt_x_yr ⟩ := hltxyr
               obtain ⟨ h4, hlt_y_xr ⟩ := hltyxr
-              obtain hleq := yjs_lt_total hxo hyo
+              obtain hleq := yjs_lt_total hxo hyo (inv := inv)
               cases hleq with
               | inr hlt =>
                 obtain ⟨ h5, hlt_yo_xr ⟩ := hlt
@@ -141,7 +142,7 @@ lemma yjs_lt_total {A : Type} {P : @ClosedPredicate A} {inv : ItemSetInvariant P
                 exists (max4 h5 h3 h2 h4 + 1 + 1)
                 right
                 apply YjsLt.ltConflict
-                apply ConflictLt.ltOriginDiff <;> try first | simp | assumption
+                apply ConflictLt.ltOriginDiff <;> try first | assumption | simp
               | inl hleq =>
                 obtain ⟨ h5, hlt_yo_xr ⟩ := hleq
                 cases hlt_yo_xr with
